code cleanup

src/Models.v
@@ -5,301 +5,310 @@ Import ListNotations.
 
 Section Models.
 
-  (* Finite bound on the number of random values you and the attacker will need. *)
+  (* Finite bound on the number of random values
+     you and the attacker will need. *)
   Context (rand_bound : nat).
   Context (arand_bound : nat).
 
-Section SymbolicModel.
+  Section SymbolicModel.
 
-  Inductive SymbolicSort :=
-  | Message : SymbolicSort
-  | Bool : SymbolicSort.
+    Inductive SymbolicSort :=
+    | Message : SymbolicSort
+    | Bool : SymbolicSort.
 
-  Inductive SymbolicFunc : list SymbolicSort -> SymbolicSort -> Type :=
-  | STrue : SymbolicFunc [] Bool
-  | SFalse : SymbolicFunc [] Bool
-  | IfThenElse : SymbolicFunc (Bool :: Message :: Message :: []) Message
-  | EmptyMsg : SymbolicFunc [] Message
-  | Eq : SymbolicFunc (Message :: Message :: []) Bool
-  | EqL : SymbolicFunc (Message :: Message :: []) Bool
-  | Name : forall (n : nat), n < rand_bound -> (SymbolicFunc [] Message)
-  | Handle : forall (n : nat) (dom : list SymbolicSort) (cod : SymbolicSort), SymbolicFunc dom cod.
+    Inductive SymbolicFunc : list SymbolicSort -> SymbolicSort -> Type :=
+    | STrue : SymbolicFunc [] Bool
+    | SFalse : SymbolicFunc [] Bool
+    | IfThenElse : SymbolicFunc (Bool :: Message :: Message :: []) Message
+    | EmptyMsg : SymbolicFunc [] Message
+    | Eq : SymbolicFunc (Message :: Message :: []) Bool
+    | EqL : SymbolicFunc (Message :: Message :: []) Bool
+    | Name : forall (n : nat), n < rand_bound -> (SymbolicFunc [] Message)
+    | Handle : forall (n : nat) (dom : list SymbolicSort) (cod : SymbolicSort),
+        SymbolicFunc dom cod.
 
-  (* Indistinguishability is defined on both messages and booleans *)
-  Inductive SymbolicPredicate : list SymbolicSort -> Type :=
+    (* Indistinguishability is defined on both messages and booleans *)
+    Inductive SymbolicPredicate : list SymbolicSort -> Type :=
     | Indist : forall (l : list SymbolicSort), SymbolicPredicate (l ++ l).
 
-End SymbolicModel.
+  End SymbolicModel.
 
-Require Import WC_PolyTime.
-Require Import Admissibility.
-Require Import Asymptotic.
-Require Import FCF.
+  Require Import Admissibility.
+  Require Import Asymptotic.
+  Require Import FCF.
+  Require Import WC_PolyTime.
 
-Require Import CrossCrypto.CompUtil.
-Require Import CrossCrypto.FirstOrder.
-Require Import CrossCrypto.FrapTactics.
-Require Import CrossCrypto.HList.
-Require Import CrossCrypto.Tuple.
+  Require Import CrossCrypto.CompUtil.
+  Require Import CrossCrypto.FirstOrder.
+  Require Import CrossCrypto.FrapTactics.
+  Require Import CrossCrypto.HList.
+  Require Import CrossCrypto.ListUtil.
+  Require Import CrossCrypto.Tuple.
 
-Section CompInterp.
+  Section CompInterp.
 
-  Context `{function_cost_model}.
-  (* TODO: actual definition of reasonable *)
-  Definition reasonable (cost : FunctionCostModel) := True.
+    Context `{function_cost_model}.
+    (* TODO: actual definition of reasonable *)
+    Definition reasonable (cost : FunctionCostModel) := True.
 
-  Context `{reasonable cost}.
+    Context `{reasonable cost}.
 
-  Definition message := {n : nat & Bvector n}.
-  Definition rands (eta : nat) := tuple (Bvector eta) rand_bound.
-  Definition arands (eta : nat) := tuple (Bvector eta) arand_bound.
-  Definition comp (S : Set) := forall (eta : nat), rands eta -> arands eta -> Comp S.
+    Definition message := {n : nat & Bvector n}.
+    Definition rands (eta : nat) := tuple (Bvector eta) rand_bound.
+    Definition arands (eta : nat) := tuple (Bvector eta) arand_bound.
+    Definition comp (S : Set) := forall (eta : nat),
+        rands eta -> arands eta -> Comp S.
 
-  Definition curry_rands_func T eta (c : rands eta -> arands eta -> Comp T) : tuple (Bvector eta) (rand_bound + arand_bound) -> Comp T.
-    intros.
-    remember (tskipn H0 rand_bound) as arand.
-    assert (rand_bound + arand_bound - rand_bound = arand_bound).
-    linear_arithmetic.
-    clear Heqarand.
-    rewrite H1 in arand.
-    refine (c (tfirstn H0 _) arand).
-    linear_arithmetic.
-  Defined.
+    Definition curry_rands_func T eta (c : rands eta -> arands eta -> Comp T)
+      : tuple (Bvector eta) (rand_bound + arand_bound) -> Comp T.
+      intros t.
+      pose proof (tskipn t rand_bound) as arand.
+      replace (rand_bound + arand_bound - rand_bound) with arand_bound
+        in arand by linear_arithmetic.
+      refine (c (tfirstn t _) arand); linear_arithmetic.
+    Defined.
 
-  Definition bind_rands T eta (c : rands eta -> arands eta -> Comp T) : Comp T :=
-    bind_tuple (curry_rands_func c).
+    Definition bind_rands T eta (c : rands eta -> arands eta -> Comp T)
+      : Comp T :=
+      bind_tuple (curry_rands_func c).
 
-  Lemma message_eq_dec : forall (m n : message), {m = n} + {m <> n}.
-    intros.
-    destruct m; destruct n.
-    cases (x ==n x0).
-    subst x.
-    cases (Bvector_eq_dec b b0).
-    subst b.
-    left.
-    congruence.
-    right.
-    intuition.
-    right.
-    congruence.
-  Defined.
+    Lemma message_eq_dec : forall (m n : message), {m = n} + {m <> n}.
+      intros m m'.
+      destruct m as [n m]; destruct m' as [n' m'].
+      cases (n ==n n').
+      - subst n'.
+        cases (Bvector_eq_dec m m').
+        + subst m'.
+          left; congruence.
+        + right; intuition.
+      - right; congruence.
+    Defined.
 
-  (* TODO : Probably shouldn't need to explicitly set and unset here *)
-  Unset Implicit Arguments.
-  Record MessageComp :=
-    mkMessageComp {
-        message_comp : comp message;
-        message_poly : admissible_oc cost (fun _ => unit) (fun _ => unit) (fun _ => message) (fun (eta : nat) =>
-                                                                                                OC_Ret unit unit (bind_rands (message_comp eta)))
-      }.
+    Record MessageComp :=
+      mkMessageComp {
+          message_comp : comp message;
+          message_poly :
+            admissible_oc cost
+                          (fun _ => unit)
+                          (fun _ => unit)
+                          (fun _ => message)
+                          (fun (eta : nat) =>
+                             OC_Ret unit unit (bind_rands (@message_comp eta)))
+        }.
 
-  Record BoolComp :=
-    mkBoolComp {
-        bool_comp : comp bool;
-        bool_poly : admissible_oc cost (fun _ => unit) (fun _ => unit) (fun _ => bool) (fun (eta : nat) => OC_Ret unit unit (bind_rands (bool_comp eta)))
-      }.
-  Set Implicit Arguments.
+    Arguments mkMessageComp {message_comp} message_poly.
 
-  Definition CompDomain (s : SymbolicSort) : Type :=
-    match s with
-    | Message => MessageComp
-    | Bool => BoolComp
-    end.
+    Record BoolComp :=
+      mkBoolComp {
+          bool_comp : comp bool;
+          bool_poly :
+            admissible_oc cost
+                          (fun _ => unit)
+                          (fun _ => unit)
+                          (fun _ => bool)
+                          (fun (eta : nat) =>
+                             OC_Ret unit unit (bind_rands (@bool_comp eta)))
+        }.
 
-  Definition poly_time T (c : comp T) :=
-    admissible_oc cost (fun _ : nat => unit) (fun _ : nat => unit) (fun _ : nat => T)
-                  (fun eta : nat => $ (bind_rands (c eta))).
+    Arguments mkBoolComp {bool_comp} bool_poly.
 
-  Ltac trivial_polynomial :=
-    unfold polynomial; exists 0%nat; exists 0%nat; exists 0%nat; unfold expnat; simpl; intros; omega.
+    Definition CompDomain (s : SymbolicSort) : Type :=
+      match s with
+      | Message => MessageComp
+      | Bool => BoolComp
+      end.
 
-  Lemma constant_polytime : forall T (eq : eq_dec T) (b : T),
-      poly_time (fun eta => (fun _ : rands eta => fun _ : arands eta => Ret eq b)).
-  Admitted.
+    Definition poly_time T (c : comp T) :=
+      admissible_oc cost
+                    (fun _ : nat => unit)
+                    (fun _ : nat => unit)
+                    (fun _ : nat => T)
+                    (fun eta : nat => $ (bind_rands (c eta))).
 
-  Definition constant_boolcomp (b : bool) : BoolComp :=
-    mkBoolComp (fun _ _ _ => Ret bool_dec b) (constant_polytime bool_dec b).
+    Ltac trivial_polynomial :=
+      unfold polynomial; exists 0%nat; exists 0%nat; exists 0%nat;
+      unfold expnat; simpl; intros; omega.
 
-  Definition constant_messagecomp (m : message) : MessageComp :=
-    mkMessageComp (fun _ _ _ => Ret message_eq_dec m) (constant_polytime message_eq_dec m).
+    Lemma constant_polytime : forall T (eq : eq_dec T) (b : T),
+        poly_time (fun eta (_ : rands eta) (_ : arands eta) =>
+                     Ret eq b).
+    Admitted.
 
-  Definition if_then_else_comp (b : comp bool) (m1 m2 : comp message) : comp message :=
-    fun (eta : nat) =>
-      fun (r : rands eta) =>
-        fun (ar : arands eta) =>
-      b' <-$ (b eta r ar);
-        (if b' then m1 else m2) eta r ar.
+    Definition constant_boolcomp (b : bool) : BoolComp :=
+      mkBoolComp (constant_polytime bool_dec b).
 
+    Definition constant_messagecomp (m : message) : MessageComp :=
+      mkMessageComp (constant_polytime message_eq_dec m).
 
-  Definition if_then_else_poly: forall (b : BoolComp) (m1 m2 : MessageComp),
-      poly_time (if_then_else_comp (bool_comp b) (message_comp m1) (message_comp m2)).
-  Admitted.
+    Definition if_then_else_comp (b : comp bool) (m1 m2 : comp message)
+      : comp message :=
+      fun (eta : nat) (r : rands eta) (ar : arands eta) =>
+        b' <-$ (b eta r ar);
+          (if b' then m1 else m2) eta r ar.
 
-  Definition if_then_else_messagecomp (b : BoolComp) (m1 m2 : MessageComp) : MessageComp :=
-    mkMessageComp (if_then_else_comp b.(bool_comp) m1.(message_comp) m2.(message_comp)) (if_then_else_poly b m1 m2).
+    Definition if_then_else_poly: forall (b : BoolComp) (m1 m2 : MessageComp),
+        poly_time (if_then_else_comp (bool_comp b)
+                                     (message_comp m1)
+                                     (message_comp m2)).
+    Admitted.
 
-  Definition message_eq (m1 m2 : message) : bool.
-    cases (message_eq_dec m1 m2).
-    exact true.
-    exact false.
-  Defined.
+    Definition if_then_else_messagecomp (b : BoolComp) (m1 m2 : MessageComp)
+      : MessageComp :=
+      mkMessageComp (if_then_else_poly b m1 m2).
 
-  Definition EqDec_message : EqDec message.
-    refine (Build_EqDec _ _).
-    intros.
-    cases (message_eq_dec x y).
-    instantiate (1 := fun m1 m2 => message_eq m1 m2).
-    split; simplify; try assumption.
-    unfold message_eq.
-    cases (message_eq_dec x y).
-    trivial.
-    contradiction.
-    split; simplify; try assumption.
-    unfold message_eq in H0.
-    cases (message_eq_dec x y); try equality.
-    equality.
-  Defined.
+    Definition message_eq (m1 m2 : message) : bool :=
+      if message_eq_dec m1 m2 then true else false.
 
-  Definition eq_comp (m1 m2 : comp message) : comp bool.
-    refine (fun (eta : nat) =>
-              fun (r : rands eta) =>
-                fun (ar : arands eta) =>
-              m1' <-$ m1 eta r ar;
-              m2' <-$ m2 eta r ar;
-              ret (m1' ?= m2')).
-    apply EqDec_message.
-  Defined.
+    Definition EqDec_message : EqDec message.
+      refine (Build_EqDec message_eq _).
+      unfold message_eq.
+      intros x y.
+      destruct (message_eq_dec x y); intuition.
+    Defined.
 
-  Definition eq_poly: forall (m1 m2 : MessageComp),
-      poly_time (eq_comp (message_comp m1) (message_comp m2)).
-  Admitted.
+    Definition eq_comp (m1 m2 : comp message) : comp bool.
+      refine (fun (eta : nat) (r : rands eta) (ar : arands eta) =>
+                m1' <-$ m1 eta r ar;
+                m2' <-$ m2 eta r ar;
+                ret (m1' ?= m2')).
+      apply EqDec_message.
+    Defined.
 
-  Definition eq_boolcomp (m1 m2 : MessageComp) : BoolComp :=
-    mkBoolComp (eq_comp m1.(message_comp) m2.(message_comp)) (eq_poly m1 m2).
+    Definition eq_poly: forall (m1 m2 : MessageComp),
+        poly_time (eq_comp (message_comp m1) (message_comp m2)).
+    Admitted.
 
-  Definition eql_comp (m1 m2 : comp message) : comp bool.
-    refine (fun (eta : nat) =>
-              fun (r : rands eta) =>
-                fun (ar : arands eta) =>
-              m1' <-$ m1 eta r ar;
-              m2' <-$ m2 eta r ar;
-              ret _).
-    destruct m1'; destruct m2'.
-    exact (x ?= x0).
-  Defined.
+    Definition eq_boolcomp (m1 m2 : MessageComp) : BoolComp :=
+      mkBoolComp (eq_poly m1 m2).
 
-  Definition eql_poly: forall (m1 m2 : MessageComp),
-      poly_time (eql_comp (message_comp m1) (message_comp m2)).
-  Admitted.
+    Definition eql_comp (m1 m2 : comp message) : comp bool.
+      refine (fun (eta : nat) (r : rands eta) (ar : arands eta) =>
+                m1' <-$ m1 eta r ar;
+                m2' <-$ m2 eta r ar;
+                ret _).
 
-  Definition eql_boolcomp (m1 m2 : MessageComp) : BoolComp :=
-    mkBoolComp (eql_comp m1.(message_comp) m2.(message_comp)) (eql_poly m1 m2).
+      destruct m1' as [x1 _]; destruct m2' as [x2 _].
+      exact (x1 ?= x2).
+    Defined.
 
-  Definition name_comp (n : nat) (H' : n < rand_bound) : comp message.
-    refine (fun (eta : nat) =>
-              fun (r : rands eta) =>
-                fun (_ : arands eta) =>
+    Definition eql_poly: forall (m1 m2 : MessageComp),
+        poly_time (eql_comp (message_comp m1) (message_comp m2)).
+    Admitted.
+
+    Definition eql_boolcomp (m1 m2 : MessageComp) : BoolComp :=
+      mkBoolComp (eql_poly m1 m2).
+
+    Definition name_comp (n : nat) (H' : n < rand_bound) : comp message.
+      refine (fun (eta : nat) (r : rands eta) (_ : arands eta) =>
                 ret (existT Bvector eta (tnth r H'))).
-    exact EqDec_message.
-  Defined.
+      exact EqDec_message.
+    Defined.
 
-  Definition name_poly: forall (n : nat) (H' : n < rand_bound),
-      poly_time (fun eta => ((name_comp H') eta)).
-  Admitted.
+    Definition name_poly: forall (n : nat) (H' : n < rand_bound),
+        poly_time (fun eta => (name_comp H') eta).
+    Admitted.
 
-  Definition name_messagecomp (n : nat) (H' : n < rand_bound) : MessageComp :=
-    mkMessageComp (name_comp H') (name_poly H').
+    Definition name_messagecomp (n : nat) (H' : n < rand_bound)
+      : MessageComp :=
+      mkMessageComp (name_poly H').
 
-  Definition arands_only T (c : comp T) :=
-    exists c' : Comp T, c = fun (eta : nat) => fun (_ : rands eta) => fun (ar : arands eta) => c'.
+    (* FIXME I don't think this says the right thing. Maybe one of these? *)
+    Definition arands_only' T (c : comp T) :=
+      exists c' : forall eta : nat, arands eta -> Comp T,
+        c = fun eta _ ar => c' eta ar.
+    (* This one seems less likely to require extensionality,
+       though could be harder to eliminate *)
+    Definition arands_only'' T (c : comp T) :=
+      forall (eta : nat) (r r' : rands eta) (ar : arands eta),
+        c eta r ar = c eta r' ar.
 
-  (* Attackers are a generator of computations that are polynomial time and only access attacker randomness. *)
-  Definition attacker := forall (n : nat) T dom (args : hlist CompDomain dom),
-      {c : comp T | poly_time c & arands_only c}.
+    Definition arands_only T (c : comp T) :=
+      exists c' : Comp T,
+        c = fun (eta : nat) (_ : rands eta) (ar : arands eta) => c'.
 
-  Definition interp_handle dom cod (att : attacker) (n : nat) (args : hlist CompDomain dom) : CompDomain cod :=
-  match cod as s return (CompDomain s) with
-  | Message => let attacker_sig := (sig_of_sig2 (att n message dom args)) in
-      mkMessageComp (proj1_sig attacker_sig) (proj2_sig attacker_sig)
-  | Bool => let attacker_sig := (sig_of_sig2 (att n bool dom args)) in
-      mkBoolComp (proj1_sig attacker_sig) (proj2_sig attacker_sig)
-  end.
+    (* Attackers are a generator of computations that are polynomial time
+       and only access attacker randomness. *)
+    Definition attacker := forall (n : nat) T dom
+                                  (args : hlist CompDomain dom),
+        {c : comp T | poly_time c & arands_only c}.
 
-  Definition CompInterpFunc (att : attacker) dom cod (f : SymbolicFunc dom cod) (args : hlist CompDomain dom) : (CompDomain cod).
-    induction f.
-    (* STrue *)
-    - exact (constant_boolcomp true).
-    (* SFalse *)
-    - exact (constant_boolcomp false).
-    (* IfThenElse *)
-    - refine (if_then_else_messagecomp _ _ _).
-      inversion args.
-      exact X.
-      inversion args.
-      inversion X0.
-      exact X1.
-      inversion args.
-      inversion X0.
-      inversion X2.
-      exact X3.
-    (* EmptyMsg *)
-    - exact (constant_messagecomp (existT Bvector 0 Bnil)%nat).
-    (* Eq *)
-    - refine (eq_boolcomp _ _).
-      inversion args.
-      exact X.
-      inversion args.
-      inversion X0.
-      exact X1.
-    (* EqL *)
-    - refine (eql_boolcomp _ _).
-      inversion args.
-      exact X.
-      inversion args.
-      inversion X0.
-      exact X1.
-    (* Name *)
-    - exact (name_messagecomp l).
-    (* Handle *)
-    - exact (interp_handle cod att n args).
-  Defined.
+    Definition interp_handle dom cod (att : attacker) (n : nat)
+               (args : hlist CompDomain dom) : CompDomain cod :=
+      match cod as s return (CompDomain s) with
+      | Message => let attacker_sig := sig_of_sig2 (att n message dom args) in
+                   mkMessageComp (proj2_sig attacker_sig)
+      | Bool => let attacker_sig := (sig_of_sig2 (att n bool dom args)) in
+                mkBoolComp (proj2_sig attacker_sig)
+      end.
 
-Definition indist_comp := forall dom, hlist CompDomain dom -> comp bool.
+    Definition CompInterpFunc (att : attacker) dom cod
+               (f : SymbolicFunc dom cod) (args : hlist CompDomain dom)
+      : (CompDomain cod).
+      induction f.
+      (* STrue *)
+      - exact (constant_boolcomp true).
+      (* SFalse *)
+      - exact (constant_boolcomp false).
+      (* IfThenElse *)
+      - refine (if_then_else_messagecomp _ _ _).
+        inversion args.
+        exact X.
+        inversion args.
+        inversion X0.
+        exact X1.
+        inversion args.
+        inversion X0.
+        inversion X2.
+        exact X3.
+      (* EmptyMsg *)
+      - exact (constant_messagecomp (existT Bvector 0 Bnil)%nat).
+      (* Eq *)
+      - refine (eq_boolcomp _ _).
+        inversion args.
+        exact X.
+        inversion args.
+        inversion X0.
+        exact X1.
+      (* EqL *)
+      - refine (eql_boolcomp _ _).
+        inversion args.
+        exact X.
+        inversion args.
+        inversion X0.
+        exact X1.
+      (* Name *)
+      - exact (name_messagecomp l).
+      (* Handle *)
+      - exact (interp_handle cod att n args).
+    Defined.
 
-(* TODO: Do we need to somehow bind_rands outside of the probability statement? I don't think so... *)
-Definition indist dom (l1 l2 : hlist CompDomain dom) : Prop :=
-  forall (f : indist_comp), poly_time (f dom l1) 
-                       -> poly_time (f dom l2)
-                       -> arands_only (f dom l1)
-                       -> arands_only (f dom l2)
-                       -> negligible (fun (eta : nat) => (| Pr[bind_rands (f dom l1 eta)] - Pr[bind_rands (f dom l2 eta)]|)).
+    Definition indist_comp := forall dom, hlist CompDomain dom -> comp bool.
 
-Lemma firstn_concat : forall A (l : list A) (l' : list A), firstn (length l) (l ++ l') = l.
-  induction l; intros; simplify; equality.
-Qed.
+    (* TODO: Do we need to somehow bind_rands
+       outside of the probability statement? I don't think so... *)
+    Definition indist dom (l1 l2 : hlist CompDomain dom) : Prop :=
+      forall (f : indist_comp),
+        poly_time (f dom l1)
+        -> poly_time (f dom l2)
+        -> arands_only (f dom l1)
+        -> arands_only (f dom l2)
+        -> negligible (fun (eta : nat) =>
+                         (| Pr[bind_rands (f dom l1 eta)] -
+                            Pr[bind_rands (f dom l2 eta)]|)).
 
-Lemma skipn_concat : forall A (l : list A) (l' : list A), skipn (length l) (l ++ l') = l'.
-  induction l; intros; simplify; equality.
-Qed.
+    Definition CompInterpPredicate dom (p : SymbolicPredicate dom)
+               (args : hlist CompDomain dom) : Prop.
+      induction p.
+      (* assert (firstn (length l) (l ++ l) = skipn (length l) (l ++ l)). *)
+      refine (indist (hfirstn (length l) args) _).
+      rewrite listdup_split.
+      exact (hskipn (length l) args).
+    Defined.
 
-Lemma listdup_split : forall A (l : list A), firstn (length l) (l ++ l) = skipn (length l) (l ++ l).
-  repeat intros.
-  rewrite (firstn_concat l l).
-  rewrite (skipn_concat l l).
-  equality.
-Qed.
+    Definition CompModel (att : attacker)
+      : model SymbolicFunc SymbolicPredicate :=
+      Model (CompInterpFunc att) CompInterpPredicate.
 
-Definition CompInterpPredicate dom (p : SymbolicPredicate dom) (args : hlist CompDomain dom) : Prop.
-  induction p.
-  (* assert (firstn (length l) (l ++ l) = skipn (length l) (l ++ l)). *)
-  refine (indist (hfirstn (length l) args) _).
-  rewrite listdup_split.
-  exact (hskipn (length l) args).
-Defined.
-
-Definition CompModel (att : attacker) : model SymbolicFunc SymbolicPredicate :=
-  Model (CompInterpFunc att) CompInterpPredicate.
-
-End CompInterp.
+  End CompInterp.
 
 End Models.
