src/ListUtil.v
@@ -21,15 +21,18 @@ Fixpoint nth_with_proof T (n:nat) (l:list T) {struct l} :
   omega.
 Defined.
 
-Lemma firstn_concat : forall A (l : list A) (l' : list A), firstn (length l) (l ++ l') = l.
+Lemma firstn_concat : forall A (l : list A) (l' : list A),
+    firstn (length l) (l ++ l') = l.
   induction l; intros; simplify; equality.
 Qed.
 
-Lemma skipn_concat : forall A (l : list A) (l' : list A), skipn (length l) (l ++ l') = l'.
+Lemma skipn_concat : forall A (l : list A) (l' : list A),
+    skipn (length l) (l ++ l') = l'.
   induction l; intros; simplify; equality.
 Qed.
 
-Lemma listdup_split : forall A (l : list A), firstn (length l) (l ++ l) = skipn (length l) (l ++ l).
+Lemma listdup_split : forall A (l : list A),
+    firstn (length l) (l ++ l) = skipn (length l) (l ++ l).
   repeat intros.
   rewrite (firstn_concat l l).
   rewrite (skipn_concat l l).
